DinD: Add a notion of valid expressions
This will allow generalized application without losing the convenience
of knowing how many arguments unary and binary operators have.

Along the way, simplifies the calc sequences in CompileExpr

Doesn’t yet propagate validity through EliminateNegatedBinops, so
there’s a dynamic check before compilation.

Source/DafnyCompilers/CSharp/Compiler.dfy
@@ -168,6 +168,16 @@ module {:extern "DafnyInDafny.CSharp"} CSharpDafnyCompiler {
               0
           }
         }
+
+      }
+
+      function method ValidExpr(e: Expr): bool {
+        match e {
+          case Apply(UnaryOp(_), es) => |es| == 1
+          case Apply(BinaryOp(_), es) => |es| == 2
+          case Invalid(_) => false
+          case _ => true
+        }
       }
 
       type t = Expr
@@ -555,6 +565,12 @@ module {:extern "DafnyInDafny.CSharp"} CSharpDafnyCompiler {
       requires Shallow.All_Program(p, (e => Deep.All_Expr(e, P)))
       ensures Deep.All_Program(p, P)
     {}
+
+    lemma AllImpliesChildren(e: Expr.t, p: Expr.t -> bool)
+      requires Deep.All_Expr(e, p)
+      ensures Deep.AllChildren_Expr(e, p)
+    {}
+
   }
 
   module Rewriter {
@@ -893,6 +909,7 @@ module {:extern "DafnyInDafny.CSharp"} CSharpDafnyCompiler {
     import Simplifier
     import Translator
     import opened AST
+    import opened AST.Expr
     import opened AST.Type
     import opened StrTree_ = StrTree
     import opened Lib.Datatypes
@@ -1038,59 +1055,43 @@ module {:extern "DafnyInDafny.CSharp"} CSharpDafnyCompiler {
     function method CompilePrint(e: Expr.t) : StrTree
       decreases e, 1
       requires All_Expr(e, Simplifier.NotANegatedBinopExpr)
+      requires All_Expr(e, Expr.ValidExpr)
     {
       StrTree_.Seq([Call(Str("DafnyRuntime.Helpers.Print"), [CompileExpr(e)]), Str(";")])
     }
 
     function method CompileExpr(e: Expr.t) : StrTree
       requires Deep.All_Expr(e, Simplifier.NotANegatedBinopExpr)
+      requires Deep.All_Expr(e, Expr.ValidExpr)
       decreases e, 0
-    { // FIXME why are the calcs needed?
+    {
+      Predicates.AllImpliesChildren(e, Simplifier.NotANegatedBinopExpr);
+      Predicates.AllImpliesChildren(e, Expr.ValidExpr);
       match e {
         case Literal(l) =>
           CompileLiteralExpr(l)
         case UnaryOp(op, e') =>
-          calc ==> {
-            Deep.All_Expr(e, Simplifier.NotANegatedBinopExpr);
-            Deep.AllChildren_Expr(e, Simplifier.NotANegatedBinopExpr);
-            Deep.All_Expr(e', Simplifier.NotANegatedBinopExpr);
-          }
           var c := CompileExpr(e');
           CompileUnaryOpExpr(op, c)
         case Binary(op, e0, e1) =>
-          calc ==> {
-            Deep.All_Expr(e, Simplifier.NotANegatedBinopExpr);
-            Deep.AllChildren_Expr(e, Simplifier.NotANegatedBinopExpr);
-            && Deep.All_Expr(e0, Simplifier.NotANegatedBinopExpr)
-            && Deep.All_Expr(e1, Simplifier.NotANegatedBinopExpr);
-          }
           var c0, c1 := CompileExpr(e0), CompileExpr(e1);
           CompileBinaryExpr(op, c0, c1)
-        case Apply(_, _) =>
-          Unsupported
+        case Apply(UnaryOp(op), es) =>
+          var c := CompileExpr(es[0]);
+          CompileUnaryOpExpr(op, c)
+        case Apply(BinaryOp(op), es) => Unsupported
+        case Apply(Function(e), es) => Unsupported
+        case Apply(ClassConstructor(classType), es) => Unsupported
+        case Apply(DataConstructor(name, typeArgs), es) => Unsupported
+        case Apply(ClassMethod(receiver, name, typeArgs), es) => Unsupported
         case Display(ty, exprs) =>
-          calc ==> {
-            Deep.All_Expr(e, Simplifier.NotANegatedBinopExpr);
-            Deep.AllChildren_Expr(e, Simplifier.NotANegatedBinopExpr);
-            Seq.All(e => Deep.All_Expr(e, Simplifier.NotANegatedBinopExpr), exprs);
-          }
           CompileDisplayExpr(ty, Lib.Seq.Map((e requires e in exprs => CompileExpr(e)), exprs))
         case Invalid(_) => Unsupported
         case UnsupportedExpr(_) => Unsupported
 
         case Block(exprs) =>
-          calc ==> {
-            Deep.All_Expr(e, Simplifier.NotANegatedBinopExpr);
-            Deep.AllChildren_Expr(e, Simplifier.NotANegatedBinopExpr);
-            Seq.All(e => Deep.All_Expr(e, Simplifier.NotANegatedBinopExpr), exprs);
-          }
           Concat("\n", Lib.Seq.Map(e requires e in exprs => CompileExpr(e), exprs))
         case Print(exprs) =>
-          calc ==> {
-            Deep.All_Expr(e, Simplifier.NotANegatedBinopExpr);
-            Deep.AllChildren_Expr(e, Simplifier.NotANegatedBinopExpr);
-            Seq.All(e => Deep.All_Expr(e, Simplifier.NotANegatedBinopExpr), exprs);
-          }
           Concat("\n", Lib.Seq.Map(e requires e in exprs => CompilePrint(e), exprs))
         case UnsupportedStmt(_) => Unsupported
       }
@@ -1098,6 +1099,7 @@ module {:extern "DafnyInDafny.CSharp"} CSharpDafnyCompiler {
 
     function method CompileMethod(m: Method) : StrTree
       requires Deep.All_Method(m, Simplifier.NotANegatedBinopExpr)
+      requires Deep.All_Method(m, Expr.ValidExpr)
     {
       match m {
         case Method(nm, methodBody) => CompileExpr(methodBody)
@@ -1106,9 +1108,21 @@ module {:extern "DafnyInDafny.CSharp"} CSharpDafnyCompiler {
 
     function method CompileProgram(p: Program) : StrTree
       requires Deep.All_Program(p, Simplifier.NotANegatedBinopExpr)
+      requires Deep.All_Program(p, Expr.ValidExpr)
     {
       match p {
         case Program(mainMethod) => CompileMethod(mainMethod)
+      }
+    }
+
+    method AlwaysCompileProgram(p: Program) returns (st: StrTree)
+      requires Deep.All_Program(p, Simplifier.NotANegatedBinopExpr)
+    {
+      // TODO: this property is tedious to propagate so isn't complete yet
+      if Deep.All_Program(p, ValidExpr) {
+        st := CompileProgram(p);
+      } else {
+        st := StrTree.Str("// Invalid program.");
       }
     }
   }
@@ -1137,7 +1151,7 @@ module {:extern "DafnyInDafny.CSharp"} CSharpDafnyCompiler {
       var st := new CSharpDafnyInterop.SyntaxTreeAdapter(wr);
       var translated := Translator.TranslateProgram(dafnyProgram);
       var lowered := Simplifier.EliminateNegatedBinops(translated);
-      var compiled := Compiler.CompileProgram(lowered);
+      var compiled := Compiler.AlwaysCompileProgram(lowered);
       WriteAST(st, compiled);
     }
 
